case_study/RiscvPmp/IrisModelBinary.v
@@ -66,14 +66,14 @@ Module RiscvPmpIrisBase2 <: IrisBase2 RiscvPmpBase RiscvPmpProgram RiscvPmpSeman
     Existing Class memGS2.
     Definition memGS2_memGS_left : forall `{mG : memGS2 Σ}, memGS Σ := @mc_ghGS2_left.
     Definition memGS2_memGS_right : forall `{mG : memGS2 Σ}, memGS Σ := @mc_ghGS2_right.
-    Definition mem_inv2 : forall {Σ}, memGS2 Σ -> Memory -> Memory -> iProp Σ :=
+    Definition mem_state_interp2 : forall {Σ}, memGS2 Σ -> Memory -> Memory -> iProp Σ :=
       fun {Σ} hG μ1 μ2 =>
         (RiscvPmpIrisBase.mem_inv memGS2_memGS_left μ1 ∗ RiscvPmpIrisBase.mem_inv memGS2_memGS_right μ2
         )%I.
     Lemma mem_inv2_mem_inv :
       forall `{mG : memGS2 Σ} (μ1 μ2 : Memory),
-        mem_inv2 mG μ1 μ2 ⊣⊢ mem_inv memGS2_memGS_left μ1 ∗ mem_inv memGS2_memGS_right μ2.
-    Proof. by unfold mem_inv2. Qed.
+        mem_state_interp2 mG μ1 μ2 ⊣⊢ mem_state_interp memGS2_memGS_left μ1 ∗ mem_state_interp memGS2_memGS_right μ2.
+    Proof. by unfold mem_state_interp2. Qed.
 
     Definition memGS2_gtGS2_left `{mG : memGS2 Σ} : traceG Trace Σ :=
       @mc_gtGS _ memGS2_memGS_left.
