case_study/RiscvPmp/BlockVer/Examples.v
@@ -38,6 +38,7 @@ From Katamaran Require Import
      RiscvPmp.BlockVer.Spec
      RiscvPmp.BlockVer.PartialVerifier
      RiscvPmp.Machine
+     RiscvPmp.trace
      RiscvPmp.Sig.
 
 Import RiscvPmpProgram.
@@ -271,7 +272,7 @@ Module Examples.
       Import RiscvPmpBlockVerifIrisInstance.
       Import RiscvPmpIrisInstanceWithContracts.
 
-      Context `{sailGS Σ} `{sailGS2 Σ}.
+      Context `{sailGS Σ} {rG : iostateG IOState Σ}.
 
       Definition ptsto_instrs_from_contract {Γ} (c : @BlockVerifierContract Γ) (a : Val ty_xlenbits) : iProp Σ :=
         ptsto_instrs a (extract_instrs_from_contract c).
